theories/iris/logrel/fundamental_kinding.v
@@ -122,15 +122,15 @@ Section FundamentalKinding.
   Qed.
 
   Lemma subst_interp_kinds_map κs s__mem s__rep s__size se :
-    sem_env_interp sr mr κs s__mem s__rep s__size se ->
+    sem_env_interp sr gci κs s__mem s__rep s__size se ->
     map fst se = map (subst_kind s__mem s__rep s__size) κs.
   Proof.
   Admitted.
 
   Theorem kinding_refinement F s__mem s__rep s__size se τ κ : 
     has_kind F τ κ ->
-    subst_env_interp sr mr F s__mem s__rep s__size se ->
-    value_interp sr mr gci se (subst_type s__mem s__rep s__size VarT τ) ⊑
+    subst_env_interp sr gci F s__mem s__rep s__size se ->
+    value_interp sr gci se (subst_type s__mem s__rep s__size VarT τ) ⊑
       kind_as_type_interp sr (subst_kind s__mem s__rep s__size κ).
   Proof.
     (*
@@ -164,12 +164,9 @@ Section FundamentalKinding.
       destruct (eval_rep r); typeclasses eauto.
   Qed.
 
-  Instance copyability_proper : Proper (eq ==> eq ==> eq ==> equiv ==> equiv) copyability_interp.
-  Admitted.
-
   Lemma value_interp_var (se: semantic_env) (t: nat) (κ: kind) (T: semantic_type) :
     se !! t = Some (κ, T) ->
-    value_interp sr mr gci se (VarT t) ≡ (λne sv, kind_as_type_interp sr κ sv ∗ T sv)%I.
+    value_interp sr gci se (VarT t) ≡ (λne sv, kind_as_type_interp sr κ sv ∗ T sv)%I.
   Proof.
     intros.
     rewrite value_interp_part_eq.
@@ -187,13 +184,13 @@ Section FundamentalKinding.
   Qed.
 
   Lemma explicit_copy_prim_reps_interp ιs :
-    explicit_copy_spec mr ιs (prim_reps_interp sr ιs).
+    explicit_copy_spec sr gci ιs (prim_reps_interp sr ιs).
   Proof.
   Admitted.
 
   Lemma copyability_kind ρ ιs χ δ :
     eval_rep ρ = Some ιs ->
-    copyability_interp mr ρ χ (kind_as_type_interp sr (VALTYPE ρ χ δ)).
+    copyability_interp sr gci ρ χ (kind_as_type_interp sr (VALTYPE ρ χ δ)).
   Proof.
     unfold copyability_interp.
     intros H.
@@ -210,9 +207,9 @@ Section FundamentalKinding.
   Qed.
 
   Lemma copyability_sep ρ χ S T :
-    copyability_interp mr ρ χ S ->
-    copyability_interp mr ρ χ T ->
-    copyability_interp mr ρ χ (λne sv, (S sv ∗ T sv)%I).
+    copyability_interp sr gci ρ χ S ->
+    copyability_interp sr gci ρ χ T ->
+    copyability_interp sr gci ρ χ (λne sv, (S sv ∗ T sv)%I).
   Proof.
     destruct χ; cbn.
     - auto.
@@ -223,8 +220,8 @@ Section FundamentalKinding.
 
   Theorem kinding_copyable F s__mem s__rep s__size se τ ρ χ δ : 
     has_kind F τ (VALTYPE ρ χ δ) ->
-    subst_env_interp sr mr F s__mem s__rep s__size se ->
-    copyability_interp mr (subst_representation s__rep ρ) χ (value_interp sr mr gci se (subst_type s__mem s__rep s__size VarT τ)).
+    subst_env_interp sr gci F s__mem s__rep s__size se ->
+    copyability_interp sr gci (subst_representation s__rep ρ) χ (value_interp sr gci se (subst_type s__mem s__rep s__size VarT τ)).
   Proof.
     intros Hkind.
     remember (VALTYPE ρ χ δ) as κ.
@@ -303,9 +300,9 @@ Section FundamentalKinding.
 
   Theorem kinding_sound F s__mem s__rep s__size se τ κ : 
     has_kind F τ κ ->
-    subst_env_interp sr mr F s__mem s__rep s__size se ->
-    kind_interp sr mr (subst_kind s__mem s__rep s__size κ)
-      (value_interp sr mr gci se (subst_type s__mem s__rep s__size VarT τ)).
+    subst_env_interp sr gci F s__mem s__rep s__size se ->
+    kind_interp sr gci (subst_kind s__mem s__rep s__size κ)
+      (value_interp sr gci se (subst_type s__mem s__rep s__size VarT τ)).
   Proof.
     intros Hkind. 
     revert s__mem s__rep s__size se.
