theories/iris/logrel/relations_module.v
@@ -19,15 +19,26 @@ Section Relations.
 
   (* TODO *)
   Definition module_interp (ω : module_type) (mr : module_runtime) (m : W.module) : iProp Σ :=
-    (∀ i,
+    (∀ i imports exports,
        i ↪[mods] m -∗
-       let exports := [] in (* TODO *)
-       let imports := [] in (* TODO *)
+       (* TODO: Assert that indices in the module point to the global runtime funcaddrs. *)
+       ([∗ list] i ↦ ϕ ∈ ω.(mt_imports),
+          ∃ bs j cl,
+            N.of_nat i ↪[vis] Build_module_export bs (MED_func j) ∗
+              N.of_nat (funcimm j) ↦[wf] cl ∗
+              closure_interp sr gci [] ϕ cl ∗
+              ⌜imports !! (funcimm mr.(mr_func_user) + i)%nat = Some (N.of_nat (funcimm j))⌝) -∗
+       ([∗ list] i ↦ '_ ∈ ω.(mt_exports),
+          ∃ bs j,
+            N.of_nat i ↪[vis] Build_module_export bs (MED_func j) ∗
+              ⌜exports !! i = Some (N.of_nat (funcimm j))⌝) -∗
        WP (([ID_instantiate exports i imports], []) : host_expr) @ top
           {{ v, ⌜v = immHV []⌝ ∗
-                i ↪[mods] m ∗
-                (* TODO: Relate instance to imports/exports. *)
-                ∃ M inst, instance_interp sr mr gci M inst }})%I.
+                  i ↪[mods] m ∗
+                  ([∗ list] i ↦ ϕ ∈ ω.(mt_exports),
+                     ∃ j cl, (* TODO: same j as precond *)
+                       N.of_nat (funcimm j) ↦[wf] cl ∗
+                         closure_interp sr gci [] ϕ cl) }})%I.
 
   (* TODO *)
   Definition has_module_type_sem (m : W.module) (ω : module_type) : iProp Σ :=
